pancake/loop_removeScript.sml
@@ -6,34 +6,6 @@ open preamble loopLangTheory
 
 val _ = new_theory "loop_remove";
 
-Definition mark_all_def:
-  (mark_all (Seq p1 p2) =
-     let (p1,t1) = mark_all p1 in
-     let (p2,t2) = mark_all p2 in
-     let t3 = (t1 /\ t2) in
-       (if t3 then Mark (Seq p1 p2) else Seq p1 p2, t3)) /\
-  (mark_all (Loop l1 body l2) =
-     let (body,t1) = mark_all body in
-       (Loop l1 body l2, F)) /\
-  (mark_all (If x1 x2 x3 p1 p2 l1) =
-     let (p1,t1) = mark_all p1 in
-     let (p2,t2) = mark_all p2 in
-     let p3 = If x1 x2 x3 p1 p2 l1 in
-     let t3 = (t1 /\ t2) in
-       (if t3 then Mark p3 else p3, t3)) /\
-  (mark_all (Mark p1) = mark_all p1) /\
-  (mark_all (Call ret dest args handler) =
-     case handler of
-     | NONE => (Mark (Call ret dest args handler), T)
-     | SOME (n,p1,p2,l) =>
-         let (p1,t1) = mark_all p1 in
-         let (p2,t2) = mark_all p2 in
-         let t3 = (t1 ∧ t2) in
-         let p3 = Call ret dest args (SOME (n,p1,p2,l)) in
-           (if t3 then Mark p3 else p3, t3)) /\
-  (mark_all prog = (Mark prog,T))
-End
-
 Definition comp_no_loop_def:
   (comp_no_loop p (Seq p1 p2) =
     Seq (comp_no_loop p p1) (comp_no_loop p p2)) /\
