pancake/semantics/pan_commonPropsScript.sml
@@ -706,4 +706,21 @@ Proof
   strip_tac >> rfs []
 QED
 
+
+Theorem lookup_some_el:
+  ∀xs n x. lookup n (fromAList xs) = SOME x ==>
+   ∃m. m < LENGTH xs ∧ EL m xs = (n,x)
+Proof
+  Induct >> rw []
+  >- fs [fromAList_def, lookup_def] >>
+  cases_on ‘h’ >> fs [] >>
+  fs [fromAList_def] >>
+  fs [lookup_insert] >>
+  every_case_tac >> fs [] >> rveq >> gs []
+  >- (
+  qexists_tac ‘0’ >> fs []) >>
+  res_tac >> fs [] >> rveq >> gs [] >>
+  qexists_tac ‘SUC m’ >> fs []
+QED
+
 val _ = export_theory();
